examples/Bank_AnalysisModel.thy
@@ -57,9 +57,11 @@ generation_syntax [ (*deep
                       (IMPORTS ["../src/UML_Main", "../src/compiler/OCL_compiler_static"]
                                "../src/compiler/OCL_compiler_generator_dynamic")
                       SECTION
+                      (*SORRY*)
                       [ in SML module_name M (no_signatures) ]
                       (output_directory "../doc")
-                  ,*) shallow (generation_semantics [ analysis ]) ]
+                  ,*) shallow (generation_semantics [ analysis ])
+                              (*SORRY*) ]
 
 Class Bank
   Attributes name : String
