examples/Employee_AnalysisModel_UMLPart_generator_deep.thy
@@ -55,6 +55,7 @@ generation_syntax [ deep
                       (IMPORTS ["../src/UML_Main", "../src/compiler/OCL_compiler_static"]
                                "../src/compiler/OCL_compiler_generator_dynamic")
                       SECTION
+                      (*SORRY*)
                       [ in SML module_name M (no_signatures) ]
                       (output_directory "../doc")
                   (*, syntax_print*) ]
